HOL: not sure about this, new def

HOL/panScript.sml
@@ -17,8 +17,6 @@ open panPtreeConversionTheory; (* parse_funs_to_ast *)
 open panItreeSemTheory panItreePropsTheory;
 (* open set_sepTheory; *)
 
-(* can only load from here XXX bug? *)
-
 val _ = temp_set_fixity "≈" (Infixl 500);
 Overload "≈" = “itree_wbisim”;
 val _ = temp_set_fixity ">>=" (Infixl 500);
@@ -107,15 +105,15 @@ Proof
   rw[miscTheory.read_bytearray_def]
 QED
 
-Theorem h_prog_skip[simp] = cj 1 h_prog_def;
 Theorem mrec_sem_simps[simp] = panItreeSemTheory.mrec_sem_simps;
 
-val assign_tac = gvs[Once h_prog_def, h_prog_assign_def, eval_def];
-val strb_tac = rw[Once h_prog_def, h_prog_store_byte_def];
+(*
+ * hmm, this is suitable for global invariants but not quite
+ *)
 
 Definition triple:
   triple inv (p,s) post =
-  (∀k. (∀a. post a ⇒ inv (k a))
+  (∀k. (∀rs. post rs ⇒ inv (k rs))
        ⇒
        inv (mrec_sem (h_prog (p,s)) >>= k))
 End
@@ -374,7 +372,104 @@ Proof
 QED
 
 (*
- * coinductive example: random register
+ * interesting, but we should try a better suited definition
+ * for describing finite trace properties of a program (fragment)
+ *)
+
+Definition next_def:
+  next tr (dev,s) (array_ptr,e)
+          (post :γ -> 32 result option -> (32, α) bstate
+                   -> (32, α) stree -> bool)
+          (t : (32, α) stree) =
+  (∀a dev'.
+     tr dev (e,a) dev' ⇒
+     (∃(k : 'a ffi_result -> (32, α) stree).
+        strip_tau t (Vis e k) ∧
+        case a of
+          FFI_final a => ARB
+        | FFI_return ffi bytes
+          => post dev' NONE
+                  (s with <|memory := write_bytearray array_ptr bytes
+                                      s.memory s.memaddrs s.be; ffi := ffi|>)
+                  (k a)))
+End
+
+val ffi_ast = parse_pancake ‘
+fun f() {
+  @read(0,0,@base,1);
+  @write(@base,1,0,0);
+}’;
+
+val ffi_noannot =
+  rhs $ concl $ SRULE[]
+      $ INST_TYPE [alpha |-> ``: 32``] $ EVAL “del_annot (fun_ast ^ffi_ast)”;
+
+Theorem test:
+  (∀(dev : 'b) r s. mem_load_byte s.memory s.memaddrs s.be s.base_addr = SOME 0w
+             ⇒ P dev r s (Tau (k (r,s)))) ∧
+  mem_load_byte s.memory s.memaddrs s.be s.base_addr = SOME b ⇒
+  next (λ_ (e,a) _. ∃ffi. a = FFI_return ffi [0w])
+       ((), s)
+       (s.base_addr, (FFI_call (ExtCall "read") [] [b]))
+       P
+       (Tau
+        (mrec_sem
+         (h_prog (ExtCall «read» (Const 0w) (Const 0w) BaseAddr (Const 1w),s))
+         >>= k))
+Proof
+  rw[h_prog_def, h_prog_ext_call_def, read_bytearray_1] >>
+  rw[next_def] >> rw[] >>
+  last_x_assum irule >> rw[] >>
+  cheat
+QED
+
+Theorem test2:
+  mem_load_byte s.memory s.memaddrs s.be s.base_addr = SOME 0w ⇒
+  next (λ_ (e,a) _. ∃ffi b. a = FFI_return ffi [0w])
+       ((), s)
+       (s.base_addr, (FFI_call (ExtCall "write") [0w] []))
+       (λdev r s t. r = NONE)
+       (mrec_sem
+        (h_prog (ExtCall «write» BaseAddr (Const 1w) (Const 0w) (Const 0w),
+                 (s : (32,'a) bstate))))
+Proof
+  rw[h_prog_def, h_prog_ext_call_def, read_bytearray_1] >>
+  rw[next_def] >> rw[]
+QED
+
+Theorem testseq:
+  mem_load_byte s.memory s.memaddrs s.be s.base_addr = SOME b ⇒
+  next (λ_ (e,a) _. ∃ffi b. a = FFI_return ffi [0w])
+       ((), s)
+       (s.base_addr, (FFI_call (ExtCall "read") [] [b]))
+       (λdev' r s' t.
+          mem_load_byte s'.memory s'.memaddrs s'.be s'.base_addr = SOME 0w ⇒
+          next (λ_ (e,a) _. ∃ffi b. a = FFI_return ffi [0w])
+               ((), s')
+               (s'.base_addr, (FFI_call (ExtCall "write") [0w] []))
+               (λdev r _ _. r = NONE)
+               t)
+       (mrec_sem (h_prog (^ffi_noannot,s)))
+Proof
+  rw[Once h_prog_def, h_prog_seq_def] >>
+  qmatch_goalsub_abbrev_tac ‘next _ _ _ P’ >>
+  rw[mrec_sem_monad_law] >>
+  qmatch_goalsub_abbrev_tac ‘mrec_sem _ >>= k’ >>
+  irule test >> simp[Abbr ‘P’, Abbr ‘k’] >>
+
+  irule test2
+QED
+
+(* coinductive example: random register
+ *
+ * note: Devices may make silent transitions and may race with the driver,
+ *       so then composition of driver and device is not then a deterministic
+ *       function of the env and so cannot represented as an itree.
+ *
+ * let's split the proof into
+ * 1) the program follows the protocol (all events have a valid device answer)
+ *    - implicit in specification, needs to be proved separately
+ * 2) the program is correct on all traces assuming the device follows protocol
  *)
 
 val reg_ast = parse_pancake ‘
@@ -386,7 +481,7 @@ fun reg() {
 }’;
 
 val reg_annot = rhs $ concl $ SRULE[]
-                    $ INST_TYPE [alpha |-> ``: 32``] $ EVAL “(fun_ast ^reg_ast)”;
+                    $ INST_TYPE [alpha |-> ``:32``] $ EVAL “(fun_ast ^reg_ast)”;
 val reg_noannot =
   rhs $ concl $ SRULE[]
       $ INST_TYPE [alpha |-> ``: 32``] $ EVAL “del_annot (fun_ast ^reg_ast)”;
@@ -397,22 +492,19 @@ Inductive rand:
   rand b (FFI_call (ffi$ExtCall "write") [a] [], FFI_return f []) a
 End
 
-(* NONE means end the interaction *)
-(* Definition resp_def: *)
-(*   resp "read" [b] = SOME (FFI_call (ffi$ExtCall "write") [b] []) ∧ *)
-(*   resp _ _ = NONE *)
-(* End *)
-
 CoInductive reg_spec:
-  (reg_spec (t : (32,'b) stree) ∧
+  (reg_spec dev (t : (32,'b) stree) ∧
    (∀b.
-      t' ≈ (Vis (FFI_call (ffi$ExtCall "read") [] [a]) k) ∧
-      k (FFI_return ffi [b]) = Vis (FFI_call (ffi$ExtCall "write") [b] [])
-                                   (λ_. t))
+      t' ≈ (Vis e1 k) ∧ e1 = (FFI_call (ffi$ExtCall "read") [] [a]) ∧
+      ∀ans. rand dev (e1,ans) dev'
+            ⇒
+            k ans = Vis e2 (λ_. t) ∧ e2 = (FFI_call (ffi$ExtCall "write") [b] []) ∧
+            rand dev' (e2,ans2) dev''
+   )
    ⇒
-   reg_spec t')
+   reg_spec dev'' t')
   ∧
-  (reg_spec t ⇒ reg_spec (Tau t))
+  (reg_spec dev t ⇒ reg_spec dev (Tau t))
 End
 
 Theorem reg_spec_tau:
